src/ArrayList.fst
@@ -1,0 +1,74 @@
+module ArrayList
+
+open Steel.Memory
+open Steel.Effect.Atomic
+open Steel.Effect
+open Steel.ArrayRef
+
+module U32 = FStar.UInt32
+
+module A = Steel.Array
+module L = FStar.List.Tot
+module US = FStar.SizeT
+module FS = FStar.FiniteSet.Base
+module AL = ArrayListGen
+
+
+(** A monomorphized version of ArrayListGen, specialized for cells of statuses, i.e., 0ul, 1ul, or 2ul.
+    We only expose the computationally relevant functions here, all the lemmas remain in ArrayListGen *)
+
+let status = v:U32.t{U32.v v < 3}
+
+let cell = AL.cell status
+
+inline_for_extraction noextract
+let null = AL.null
+inline_for_extraction noextract
+let null_ptr = AL.null_ptr
+
+unfold
+let varraylist (pred1 pred2 pred3: status -> prop) (r:A.array cell) (hd1 hd2 hd3:nat) : vprop =
+  AL.varraylist pred1 pred2 pred3 r hd1 hd2 hd3
+
+/// Removes the element at offset [idx] from the dlist pointed to by [hd1]
+let remove1
+  (#pred1 #pred2 #pred3: status -> prop)
+  (r:A.array cell)
+  (hd1:US.t)
+  (hd2 hd3:Ghost.erased nat)
+  (idx:US.t{US.v idx < A.length r})
+   : Steel US.t
+          (varraylist pred1 pred2 pred3 r (US.v hd1) hd2 hd3)
+          (fun hd' -> varraylist pred1 pred2 pred3 r (US.v hd') hd2 hd3)
+          (requires fun h -> AL.mem (US.v idx) (US.v hd1) (h (varraylist pred1 pred2 pred3 r (US.v hd1) hd2 hd3)))
+          (ensures fun h0 hd' h1 ->
+            AL.ptrs_in (US.v hd') (h1 (varraylist pred1 pred2 pred3 r (US.v hd') hd2 hd3)) ==
+            FS.remove (US.v idx) (AL.ptrs_in (US.v hd1) (h0 (varraylist pred1 pred2 pred3 r (US.v hd1) hd2 hd3))) /\
+            AL.ptrs_in hd2 (h1 (varraylist pred1 pred2 pred3 r (US.v hd') hd2 hd3)) ==
+            AL.ptrs_in hd2 (h0 (varraylist pred1 pred2 pred3 r (US.v hd1) hd2 hd3)) /\
+            AL.ptrs_in hd3 (h1 (varraylist pred1 pred2 pred3 r (US.v hd') hd2 hd3)) ==
+            AL.ptrs_in hd3 (h0 (varraylist pred1 pred2 pred3 r (US.v hd1) hd2 hd3))
+          )
+  = AL.remove1 r hd1 hd2 hd3 idx
+
+let insert3
+  (#pred1 #pred2 #pred3: status -> prop)
+  (r:A.array cell)
+  (hd:US.t{hd == null_ptr \/ US.v hd < A.length r})
+  (hd1 hd2:Ghost.erased nat)
+  (idx:US.t{idx <> null_ptr /\ US.v idx < A.length r})
+  (v: status)
+   : Steel unit
+          (varraylist pred1 pred2 pred3 r hd1 hd2 (US.v hd))
+          (fun _ -> varraylist pred1 pred2 pred3 r hd1 hd2 (US.v idx))
+          (requires fun h -> pred3 v /\
+            (~ (AL.mem_all (US.v idx) hd1 hd2 (US.v hd) (h (varraylist pred1 pred2 pred3 r hd1 hd2 (US.v hd))))))
+          (ensures fun h0 hd' h1 ->
+            AL.ptrs_in (US.v idx) (h1 (varraylist pred1 pred2 pred3 r hd1 hd2 (US.v idx))) ==
+            FS.insert (US.v idx) (AL.ptrs_in (US.v hd) (h0 (varraylist pred1 pred2 pred3 r hd1 hd2 (US.v hd)))) /\
+            AL.ptrs_in hd1 (h1 (varraylist pred1 pred2 pred3 r hd1 hd2 (US.v idx))) ==
+            AL.ptrs_in hd1 (h0 (varraylist pred1 pred2 pred3 r hd1 hd2 (US.v hd))) /\
+            AL.ptrs_in hd2 (h1 (varraylist pred1 pred2 pred3 r hd1 hd2 (US.v idx))) ==
+            AL.ptrs_in hd2 (h0 (varraylist pred1 pred2 pred3 r hd1 hd2 (US.v hd)))
+          )
+  = AL.insert3 r hd  hd1 hd2 idx v
